

# Tutorial VIII - Exercise sheet 7

Exercise 1 : Show that if  $Y_n \rightarrow Y$  in  $L^p$ ,  $1 \leq p \leq \infty$ , then  $E(Y_n | \mathcal{G}) \rightarrow E(Y | \mathcal{G})$  in  $L^p$ .

Recall that  $\|\cdot\|_p$  is convex for  $1 \leq p \leq \infty$  (with  $p = \infty$  denoting the ess sup norm.)

Therefore,

$$\begin{aligned} \|E(Y_n | \mathcal{G}) - E(Y | \mathcal{G})\|_{L^p} &= E \|E(Y_n | \mathcal{G}) - E(Y | \mathcal{G})\|_p^p \\ &= E \|E(Y_n - Y | \mathcal{G})\|_p^p \leq E (E(|Y_n - Y|^p | \mathcal{G})) \\ &= E |Y_n - Y|^p = \|Y_n - Y\|_{L^p}^p \rightarrow 0, \text{ as } n \rightarrow \infty. \end{aligned}$$

Exercise 2 Let  $T_a = \inf\{t : B_t = a\}$ ,  $a \geq 0$ , then prove that  $E^0 \exp(-\lambda T_a) = \exp\{-a\sqrt{2\lambda}\}$

Recall that  $M_t = e^{\sigma X_t - \frac{1}{2}\sigma^2 t}$  is a  $\mathcal{F}_t$ -m.g.f.  $\sigma$

Moreover,  $T_a$  is an  $\mathcal{F}_t$ -stopping time  $\Rightarrow T_{a \wedge t}$  is a bounded stopp. time  $\forall t \geq 0$ . Assume that  $a \geq 0$

$$\text{Hence } E^0 M_{T_{a \wedge t}} = E^0 M_0 = 1,$$

$$\text{where } E^0 M_{T_{a \wedge t}} = E^0 \exp\{\sigma X_{T_{a \wedge t}} - \frac{1}{2}\sigma^2 (T_{a \wedge t})\} = 1$$

Taking  $t \rightarrow \infty$  by BCT ( $a \geq 0$ ), we have

$$\text{LHS} \rightarrow E^0 \exp\{\sigma X_{T_a} - \frac{1}{2}\sigma^2 T_a\} = E \exp\{\sigma a - \frac{1}{2}\sigma^2 T_a\} = 1$$

$$\text{Setting } \frac{\sigma^2}{2} = \lambda \geq 0, \text{ or } \sigma = \sqrt{2\lambda}, \text{ we get } E^0 \exp\{-\lambda T_a\} = \exp\{-a\sqrt{2\lambda}\}$$

Exercise 3 :  $T = \inf \{t \geq 0 : X_t \notin (-a, a)\}$

Find a Mgle of the form  $X_t^6 - C_1 t X_t^4 + C_2 t^2 X_t^2 - C_3 t^3$  and use it to calculate  $\mathbb{E}_0 T^3$ .

Recall the following lemma: (Thm 7.5.5 in Durrett)  $u(t, x)$  is a polynomial in  $t$  and  $x$ .

Solving  $\frac{\partial u}{\partial t} + \frac{1}{2} \frac{\partial^2 u}{\partial x^2} = 0$ . Then  $u(t, X_t)$  is a Mgle.

$$\text{let } u(t, x) = x^6 - C_1 t x^4 + C_2 t^2 x^2 - C_3 t^3.$$

$$\text{Then } \frac{\partial u}{\partial t} = -C_1 x^4 + 2C_2 t x^2 - 3C_3 t^2$$

$$\frac{\partial u}{\partial x} = 6x^5 - 4C_1 t x^3 + 2C_2 t^2 x$$

$$\frac{\partial^2 u}{\partial x^2} = 30x^4 - 12C_1 t x^2 + 2C_2 t^2$$

$$\text{Then, } \frac{\partial u}{\partial t} + \frac{1}{2} \frac{\partial^2 u}{\partial x^2} = -C_1 x^4 + 2C_2 t x^2 - 3C_3 t^2$$

$$+ 15x^4 - 6C_1 t x^2 + C_2 t^2$$

$$= (15 - C_1) x^4 + (2C_2 t - 6C_1 t) x^2 + (C_2 - 3C_3) t^2$$

and by setting this  $= 0$ , we get

$$\begin{cases} C_1 = 15 \\ 2C_2 - 6C_1 = 0 \Rightarrow C_2 = 3C_1 = 45 \\ C_2 - 3C_3 = 0 \Rightarrow C_3 = \frac{C_2}{3} = 15 \end{cases}$$

Then,  $X_t^6 - 15t X_t^4 + 45t^2 X_t^2 - 15t^3$  is an  $\mathbb{F}_t$ -mgle.

Therefore  $\mathbb{E}_0 u(t \wedge T, X_{t \wedge T}) = \mathbb{E}_0 u(0, X_0)$ , since  $t \wedge T$  is a bold stopping time.

Then  $0 = \mathbb{E} X_{T \wedge t}^6 - 15 \mathbb{E}(T \wedge t) X_{T \wedge t}^4 + 45 \mathbb{E}(T \wedge t)^2 X_{T \wedge t}^2 - 15 \mathbb{E}(T \wedge t)^3$   
 $X_T = (a)$   
 $= a^6 - 15 a^4 \mathbb{E}(T \wedge t) + 45 a^2 \mathbb{E}(T \wedge t)^2 - 15 \mathbb{E}(T \wedge t)^3$

$$\Rightarrow \mathbb{E}_0(T \wedge t)^3 = \frac{1}{15} \left( a^6 - 15 a^4 \mathbb{E}(T \wedge t) + 45 a^2 \mathbb{E}(T \wedge t)^2 \right) (*)$$

we must calculate  $\mathbb{E}_0(T \wedge t)$ ,  $\mathbb{E}_0(T \wedge t)^2$ .

- Note that  $\mathbb{E}_0(X_t^2 | \mathcal{F}_s) = \mathbb{E}_0((X_t - X_s) + X_s)^2 | \mathcal{F}_s$

$$\Rightarrow \mathbb{E}_0((X_t - X_s)^2 | \mathcal{F}_t) + \mathbb{E}_0(X_s^2 | \mathcal{F}_s) + 2 \mathbb{E}_0((X_t - X_s) X_s | \mathcal{F}_t)$$

$$= (t-s) + X_s^2 \Rightarrow \mathbb{E}_0(X_t^2 - t | \mathcal{F}_t) = X_s^2 - s$$

This suggests that  $X_t^2 - t$  is an  $\mathcal{F}_t$ -mgle.

Therefore  $\mathbb{E}_0(X_{T \wedge t}^2 - T \wedge t) = 0 \Rightarrow \mathbb{E}_0(T \wedge t) = \mathbb{E}_0(X_{T \wedge t}^2)$   
 $\downarrow \text{MCT} \quad \downarrow \text{BCT}$   
 $\mathbb{E}_0 T \quad a^2$

Therefore  $\mathbb{E}_0 T = a^2$  (\*\*)

- For  $\mathbb{E}(T \wedge t)^2$ , we must find a different martingale.

Claim:  $X_{T \wedge t}^4 - 6(T \wedge t) X_{T \wedge t}^2 + 3(T \wedge t)^2$

is an  $\mathcal{F}_t$ -mgle. We check this using the Lemma.

we have  $u(t, x) = x^4 - 6t x^2 + 3t^2$ . Then

$$\frac{\partial u}{\partial t} + \frac{1}{2} \frac{\partial^2 u}{\partial x^2} = -6x^2 + 6t + \frac{1}{2} [12x^2 - 12t] = 0$$

$\Rightarrow u(T \wedge t, X_{T \wedge t})$  is a Mgle

Then, we get  $\mathbb{E}_0 u(0, X_0) = 0 = \mathbb{E}_0 u(T \wedge t, X_{T \wedge t})$

$$\Rightarrow -3 \mathbb{E}_0(T \wedge t)^2 = \mathbb{E}_0(X_{T \wedge t}^4) - 6 \mathbb{E}_0((T \wedge t) X_{T \wedge t}^2)$$

We know that  $\mathbb{E}_0 T^2 = a^2 < \infty$

Then, as  $t \rightarrow \infty$ ,  $\mathbb{E}_0 (T \wedge t)^2 \rightarrow \mathbb{E}_0 T^2$  by MCT

$\mathbb{E}_0 (X_{T \wedge t})^4 \rightarrow \mathbb{E}_0 X_T^4 = a^4$  by BCT

$\mathbb{E}_0 ((T \wedge t) X_{T \wedge t}^2) \rightarrow \mathbb{E}_0 T \cdot X_T^2$  by DCT

and moreover  $\mathbb{E}_0 T \cdot X_T^2 = a^2 \mathbb{E}_0 T = a^4$ .

Combining these we get  $\mathbb{E}_0 T^2 = -\frac{1}{3} [a^4 - 6a^4] = \frac{5}{3} a^4$  (\*\*\*)

Now Combining (\*), (\*\*), (\*\*\*) and sending  $t \rightarrow \infty$  with DCT,

$$\mathbb{E}_0 T^3 = \frac{1}{15} [a^6 - 15a^4 \cdot a^2 + 45 \cdot a^2 \cdot \frac{5}{3} \cdot a^4]$$

$$= \frac{1}{15} [a^6 - 15a^6 + 75a^6] = \frac{1}{15} [61a^6] = \frac{61}{15} a^6$$



Exercise 4: show that  $t \mapsto X_t(\omega)$  are a.s. well non differentiable.

(Dvoretzky - Erdős - Kakutani, '61)

Set,  $n \geq 1$ ,  $A_n = \{\omega \in \Omega : X(\omega) \text{ is nowhere diff in } [0, n]\}$

we don't know if  $A_n$  is measurable, so we show that  $\Omega \setminus A_n \subseteq N_n$ , for some null set  $N_n$ .

Assume that  $X$  is differentiable at  $t_0 \in [0, n]$ . Then

$X$  is continuous at  $t_0 \Rightarrow \exists \delta > 0, L > 0$  s.t.  $\forall t \in B(t_0, \delta)$

$$|X(t) - X(t_0)| \leq L|t - t_0|$$

Consider the grid of  $[0, n]$   $\{j/k, j=1, \dots, nk\}$  and  $\exists k$  large enough s.t.

$$t_0 \leq j/k \quad \text{and} \quad j/k, j+1/k, j+2/k, j+3/k \in B(t_0, \delta)$$

In particular, for  $r = j+1, j+2, j+3$ :

$$\begin{aligned} |X(r/k) - X(r-1/k)| &\leq |X(r/k) - X(t_0)| + |X(t_0) - X(r-1/k)| \\ &\leq L(|r/k - t_0| + |t_0 - r-1/k|) \\ &\leq L(4/k + 3/k) = 7 \frac{L}{k} \end{aligned}$$

$$\text{Define } C_m^L = \bigcap_{n=m}^{\infty} \bigcup_{j=1}^{kn} \bigcap_{r=j+1}^{j+3} \left\{ |X(r/k) - X(r-1/k)| \leq \frac{7L}{k} \right\}$$

$$\text{Then } \Omega \setminus A_n \subseteq \bigcup_{L=1}^{\infty} \bigcup_{m=1}^{\infty} C_m^L$$

If  $W^0(C_m^L) = 0$  for all  $m, L \geq 1$  we are done.

for  $k \geq m$ ,

$$\begin{aligned}
 \mathbb{P}^0(C_m^L) &\leq \mathbb{P}^0\left(\bigcup_{j=1}^{kn} \bigcap_{r=j+1}^{j+3} \{ |X(r/k) - X(r-1/k)| \leq \frac{7L}{k} \}\right) \\
 &\leq \sum_{j=1}^{kn} \mathbb{P}^0\left(\bigcap_{r=j+1}^{j+3} \{ |X(r/k) - X(r-1/k)| \leq \frac{7L}{k} \}\right) \\
 &\stackrel{\text{indep.}}{\leq} \sum_{j=1}^{kn} \prod_{r=j+1}^{j+3} \mathbb{P}^0\left(|X(r/k) - X(r-1/k)| \leq 7L/k\right) \\
 &\stackrel{\text{stat.}}{=} \sum_{j=1}^{kn} \left(\mathbb{P}^0\left(|X(1/k)| \leq 7L/k\right)\right)^3 \\
 &\leq kn \cdot \left(\mathbb{P}^0\left(|X(1/k)| \leq 7L/k\right)\right)^3
 \end{aligned}$$

Now  $\mathbb{P}^0\left(|X(1/k)| \leq 7L/k\right) = \mathbb{P}^0\left(|X(1)| \leq \frac{7L}{\sqrt{k}}\right) = \frac{1}{\sqrt{2\pi}} \int_{-\frac{7L}{\sqrt{k}}}^{\frac{7L}{\sqrt{k}}} e^{-x^2/2} dx$   
 $X(1/k) \stackrel{d}{=} \frac{X(1)}{\sqrt{k}}$   $11 \quad -\frac{7L}{\sqrt{k}} \leq 1$

$\frac{2 \cdot 7L}{\sqrt{2\pi}} \cdot \frac{1}{\sqrt{k}}$

$$\begin{aligned}
 \text{Therefore } \mathbb{P}^0(C_m^L) &\leq k \cdot n \cdot \left( \frac{14L}{\sqrt{2\pi}} \cdot \frac{1}{\sqrt{k}} \right)^3 \\
 &= n \cdot \left( \frac{14L}{\sqrt{2\pi}} \right)^3 \cdot \frac{1}{\sqrt{k}} \rightarrow 0, \text{ as } k \rightarrow \infty.
 \end{aligned}$$

Since  $\forall \varepsilon > 0$  we can find  $k$  large enough s.t.

$$\mathbb{P}^0(C_m^L) \leq n \cdot \left( \frac{14L}{\sqrt{2\pi}} \right)^3 \cdot \frac{1}{\sqrt{k}} < \varepsilon \Rightarrow \mathbb{P}^0(C_m^L) = 0$$

$\Rightarrow e \setminus A_n$  is a null event

$\Rightarrow A_n$  is an a.s. event.